Impl.Trees.Rotate.fst
@@ -7,75 +7,15 @@ open Steel.Effect.Atomic
 open Steel.Effect
 open Steel.Reference
 
-//module Spec = Trees
 module U = FStar.UInt64
 module I = FStar.Int64
 
+open Spec.Trees
 open Impl.Core
 open Impl.Common
 open Impl.Trees
 
 #set-options "--fuel 0 --ifuel 0 --ide_id_info_off"
-
-// TODO : please prettify output after squash equiv...
-//#push-options "--ifuel 1 --fuel 2 --z3rlimit 200"
-(*
-let rotate_left (#a: Type) (ptr: t a)
-  : Steel (t a)
-  (linked_tree ptr)
-  (fun ptr' -> linked_tree ptr')
-  (requires fun h0 -> Some? (Spec.rotate_left (v_linked_tree ptr h0)))
-  (ensures (fun h0 ptr' h1 ->
-    Spec.rotate_left_wds (v_linked_tree ptr h0) == Some (v_linked_tree ptr' h1)
-  ))
-  =
-  let h0 = get () in
-  Spec.rotate_left_size (v_linked_tree ptr h0);
-  assert (Spec.size_of_tree (Spec.get (Spec.rotate_left_wds (v_linked_tree ptr h0)))
-  == Spec.size_of_tree (v_linked_tree ptr h0));
-  (**) node_is_not_null ptr;
-  (**) let x_node = unpack_tree ptr in
-  let x = get_data x_node in
-  // let ptr2 = get_right x_node in
-  // TODO : node_is_not_null ptr2 should work
-  (**) node_is_not_null (get_right x_node);
-  (**) let z_node = unpack_tree (get_right x_node) in
-  let z = get_data z_node in
-  //let h1 = get () in
-  //let t1 = v_linked_tree (get_left x_node) h1 in
-  //let t2 = v_linked_tree (get_left z_node) h1 in
-  //let t3 = v_linked_tree (get_right z_node) h1 in
-  let s1 = sot_wds (get_left x_node) in
-  let s2 = sot_wds (get_left z_node) in
-  let sx = U.add (U.add s1 s2) one in
-  //assert (U.v sx == (U.v s1) + (U.v s2) + 1);
-  //assert (U.v s1 = Spec.sot_wds (v_linked_tree (get_left x_node) h1));
-  //assert (U.v s2 = Spec.sot_wds (v_linked_tree (get_left z_node) h1));
-  write (get_size z_node) sx;
-  let tx = mk_node x (get_left x_node) (get_left z_node) (get_size z_node) in
-  write ptr tx;
-  //let h = get () in
-  //assert (fst (Spec.is_wds (v_linked_tree ptr h)));
-  //assert (U.v (sel (get_size z_node) h) == Spec.size_of_tree (v_linked_tree (get_left x_node) h)
-                                  //+ Spec.size_of_tree (v_linked_tree (get_left z_node) h) + 1);
-  //let h = get () in
-  //assert (fst (Spec.is_wds (v_linked_tree ptr h)));
-  pack_tree ptr (get_left x_node) (get_left z_node) (get_size z_node);
-  let tz = mk_node z ptr (get_right z_node) (get_size x_node) in
-  write (get_right x_node) tz;
-  //let h2 = get() in
-  //let t1' = v_linked_tree (get_left x_node) h2 in
-  //let h = get () in
-  //assert (fst (Spec.is_wds (v_linked_tree (get_right x_node) h)));
-  //assert (sel (get_size x_node) h == Spec.size_of_tree (v_linked_tree ptr h)
-  //                                 + Spec.size_of_tree (v_linked_tree (get_right z_node) h) + 1);
-  pack_tree (get_right x_node) ptr (get_right z_node) (get_size x_node);
-  //let h1 = get () in
-  //assert (Spec.size_of_tree (v_linked_tree ptr h1) == Spec.size_of_tree (v_linked_tree ptr h0));
-  return (get_right x_node)
-*)
-//(*)
-//#push-options "--ifuel 1 --fuel 2"
 
 //@Trees (rotate*)
 #push-options "--fuel 1 --ifuel 1 --z3rlimit 25"
@@ -85,19 +25,19 @@ let rotate_left (#a: Type) (ptr: t a)
   (fun ptr' -> linked_tree ptr')
   (requires (fun h0 ->
     let t = v_linked_tree ptr h0 in
-    let r = Spec.rotate_left_wdm t in
+    let r = rotate_left_wdm t in
     Some? r /\
-    Spec.height_of_tree (Spec.get r) <= Spec.height_of_tree t
+    height_of_tree (opt_get r) <= height_of_tree t
   ))
 
   (ensures (fun h0 ptr' h1 ->
-    Spec.rotate_left_wdm (v_linked_tree ptr h0)
+    rotate_left_wdm (v_linked_tree ptr h0)
     == Some (v_linked_tree ptr' h1)
   ))
   =
   let h = get () in
-  assert (Spec.size_of_tree (v_linked_tree ptr h) <= c);
-  Spec.rotate_left_size (v_linked_tree ptr h);
+  assert (size_of_tree (v_linked_tree ptr h) <= c);
+  rotate_left_size (v_linked_tree ptr h);
   (**) node_is_not_null ptr;
   (**) let x_node = unpack_tree ptr in
   let x = get_data x_node in
@@ -137,18 +77,18 @@ let rotate_right (#a: Type) (ptr: t a)
   (fun ptr' -> linked_tree ptr')
   (requires (fun h0 ->
     let t = v_linked_tree ptr h0 in
-    let r = Spec.rotate_right_wdm t in
+    let r = rotate_right_wdm t in
     Some? r /\
-    Spec.height_of_tree (Spec.get r) <= Spec.height_of_tree t
+    height_of_tree (opt_get r) <= height_of_tree t
   ))
   (ensures (fun h0 ptr' h1 ->
-    Spec.rotate_right_wdm (v_linked_tree ptr h0)
+    rotate_right_wdm (v_linked_tree ptr h0)
     == Some (v_linked_tree ptr' h1)
   ))
   =
   let h = get () in
-  assert (Spec.size_of_tree (v_linked_tree ptr h) <= c);
-  Spec.rotate_right_size (v_linked_tree ptr h);
+  assert (size_of_tree (v_linked_tree ptr h) <= c);
+  rotate_right_size (v_linked_tree ptr h);
   (**) node_is_not_null ptr;
   (**) let x_node = unpack_tree ptr in
   let x = get_data x_node in
