Spec.Trees.fst
@@ -123,7 +123,7 @@ let int_of_bool b : nat = match b with
   | false -> 0
 
 //@Trees.Misc
-let get (#a: Type) (v: option a{Some? v}) : a =
+let opt_get (#a: Type) (v: option a{Some? v}) : a =
   let Some v' = v in v'
 
 //@Trees
@@ -277,23 +277,23 @@ let rotate_left_right_wdm (#a: Type) (r: wdm a) : option (wdm a) =
 let rotate_left_size (#a: Type) (r: wdm a)
   : Lemma
   (requires Some? (rotate_left_wdm r))
-  (ensures size_of_tree (get (rotate_left_wdm r)) == size_of_tree r)
+  (ensures size_of_tree (opt_get (rotate_left_wdm r)) == size_of_tree r)
   = ()
 let rotate_right_size (#a: Type) (r: wdm a)
   : Lemma
   (requires Some? (rotate_right_wdm r))
-  (ensures size_of_tree (get (rotate_right_wdm r)) == size_of_tree r)
+  (ensures size_of_tree (opt_get (rotate_right_wdm r)) == size_of_tree r)
   = ()
 let rotate_right_left_size (#a: Type) (r: wdm a)
   : Lemma
   (requires Some? (rotate_right_left_wdm r))
   (ensures
-  size_of_tree (get (rotate_right_left_wdm r)) == size_of_tree r)
+  size_of_tree (opt_get (rotate_right_left_wdm r)) == size_of_tree r)
   = ()
 let rotate_left_right_size (#a: Type) (r: wdm a)
   : Lemma
   (requires Some? (rotate_left_right_wdm r))
   (ensures
-  size_of_tree (get (rotate_left_right_wdm r)) == size_of_tree r)
+  size_of_tree (opt_get (rotate_left_right_wdm r)) == size_of_tree r)
   = ()
 
